Lean: Specify authz response includes ids of erroring policies

cedar-lean/Cedar/Spec/Authorizer.lean
@@ -27,6 +27,13 @@ open Effect
 def satisfied (policy : Policy) (req : Request) (entities : Entities) : Bool :=
   (evaluate policy.toExpr req entities) = .ok true
 
+/--
+  Despite its name, this function is not just a version of `satisfied` that takes
+  into account the `effect`.
+
+  While `satisfied` returns Bool, `satisfiedWithEffect` returns `Option PolicyID`
+  with the policy's id if it is satisfied.
+-/
 def satisfiedWithEffect (effect : Effect) (policy : Policy) (req : Request) (entities : Entities) : Option PolicyID :=
   if policy.effect == effect && satisfied policy req entities
   then some policy.id
@@ -35,11 +42,28 @@ def satisfiedWithEffect (effect : Effect) (policy : Policy) (req : Request) (ent
 def satisfiedPolicies (effect : Effect) (policies : Policies) (req : Request) (entities : Entities) : Set PolicyID :=
   Set.make (policies.filterMap (satisfiedWithEffect effect · req entities))
 
+def hasError (policy : Policy) (req : Request) (entities : Entities) : Bool :=
+  match (evaluate policy.toExpr req entities) with
+  | .ok _ => false
+  | .error _ => true
+
+/--
+  This function is analogous to `satisfiedWithEffect` in that it returns
+  `Option PolicyID`, but not analogous to `satisfiedWithEffect` in that it does
+  not consider the policy's effect.
+-/
+def idIfHasError (policy : Policy) (req : Request) (entities : Entities) : Option PolicyID :=
+  if hasError policy req entities then some policy.id else none
+
+def errorPolicies (policies : Policies) (req : Request) (entities : Entities) : Set PolicyID :=
+  Set.make (policies.filterMap (idIfHasError · req entities))
+
 def isAuthorized (req : Request) (entities : Entities) (policies : Policies) : Response :=
   let forbids := satisfiedPolicies .forbid policies req entities
   let permits := satisfiedPolicies .permit policies req entities
+  let error_policies := errorPolicies policies req entities
   if forbids.isEmpty && !permits.isEmpty
-  then { decision := .allow, policies := permits }
-  else { decision := .deny,  policies := forbids }
+  then { decision := .allow, determining_policies := permits, error_policies }
+  else { decision := .deny,  determining_policies := forbids, error_policies }
 
 end Cedar.Spec
