cedar-lean/Cedar/Thm/Authorization/Authorizer.lean
@@ -15,7 +15,11 @@
 -/
 
 import Cedar.Spec
+import Cedar.Spec.Authorizer
 import Cedar.Thm.Authorization.Evaluator
+import Cedar.Thm.Core.LT
+import Cedar.Thm.SlicingDefs
+import Cedar.Thm.Validation.Typechecker.BinaryApp -- mapM'_asEntityUID_eq_entities
 
 /-!
 This file contains useful lemmas about the `Authorizer` functions.
@@ -26,6 +30,16 @@ namespace Cedar.Thm
 open Cedar.Spec
 open Cedar.Data
 
+theorem if_hasError_then_exists_error {policy : Policy} {request : Request} {entities : Entities} :
+  hasError policy request entities →
+  ∃ err, evaluate policy.toExpr request entities = .error err
+:= by
+  intro h₁
+  unfold hasError at h₁
+  split at h₁
+  case h_1 => simp at h₁
+  case h_2 err h₂ => exact Exists.intro err h₂
+
 theorem if_satisfied_then_satisfiedPolicies_non_empty (effect : Effect) (policies : Policies) (request : Request) (entities : Entities) :
   (∃ policy,
     policy ∈ policies ∧
@@ -33,18 +47,15 @@ theorem if_satisfied_then_satisfiedPolicies_non_empty (effect : Effect) (policie
     satisfied policy request entities) →
   (satisfiedPolicies effect policies request entities).isEmpty = false
 := by
-  intro h0
-  cases h0
-  case intro policy h1 =>
-    have ⟨ha, hb, hc⟩ := h1
-    unfold satisfiedPolicies
-    rw [←Set.make_non_empty]
-    apply @List.ne_nil_of_mem _ policy.id
-    simp [List.mem_filterMap]
-    apply Exists.intro policy
-    unfold satisfiedWithEffect
-    simp [ha, hb, hc]
-
+  intro h₀
+  replace ⟨policy, h₀⟩ := h₀
+  unfold satisfiedPolicies
+  rw [←Set.make_non_empty]
+  apply @List.ne_nil_of_mem _ policy.id
+  rw [List.mem_filterMap]
+  apply Exists.intro policy
+  unfold satisfiedWithEffect
+  simp [h₀]
 
 theorem if_satisfiedPolicies_non_empty_then_satisfied (effect : Effect) (policies : Policies) (request : Request) (entities : Entities) :
   (satisfiedPolicies effect policies request entities).isEmpty = false →
@@ -54,19 +65,21 @@ theorem if_satisfiedPolicies_non_empty_then_satisfied (effect : Effect) (policie
     satisfied policy request entities
 := by
   unfold satisfiedPolicies
-  intro h0
-  rw [←Set.make_non_empty] at h0
-  have ⟨pid, h1⟩ := List.exists_mem_of_ne_nil _ h0
-  rw [List.mem_filterMap] at h1
-  have ⟨policy, h1, h2⟩ := h1
-  unfold satisfiedWithEffect at h2
+  intro h₀
+  rw [←Set.make_non_empty] at h₀
+  have ⟨pid, h₁⟩ := List.exists_mem_of_ne_nil _ h₀
+  rw [List.mem_filterMap] at h₁
+  replace ⟨policy, h₁, h₂⟩ := h₁
+  unfold satisfiedWithEffect at h₂
   apply Exists.intro policy
-  simp [h1]
-  cases h3 : (policy.effect == effect) <;> simp at h3; simp [h3] at h2
-  simp [h3]
-  cases h4 : (satisfied policy request entities)
-  case _ => simp [h3, h4] at h2
-  case _ => rfl
+  simp [h₁]
+  cases h₃ : (policy.effect == effect) <;> simp at h₃
+  case false => simp [h₃] at h₂
+  case true =>
+    simp [h₃]
+    cases h₄ : (satisfied policy request entities) with
+    | true => rfl
+    | false => simp [h₃, h₄] at h₂
 
 theorem satisfiedPolicies_order_and_dup_independent (effect : Effect) (request : Request) (entities : Entities) (policies₁ policies₂ : Policies) :
   policies₁ ≡ policies₂ →
@@ -77,38 +90,161 @@ theorem satisfiedPolicies_order_and_dup_independent (effect : Effect) (request :
   apply Set.make_eq_if_eqv
   exact List.filterMap_equiv (satisfiedWithEffect effect · request entities) policies₁ policies₂ h₁
 
+theorem errorPolicies_order_and_dup_independent (request : Request) (entities : Entities) (policies₁ policies₂ : Policies) :
+  policies₁ ≡ policies₂ →
+  errorPolicies policies₁ request entities = errorPolicies policies₂ request entities
+:= by
+  intro h₁
+  unfold errorPolicies
+  apply Set.make_eq_if_eqv
+  exact List.filterMap_equiv (idIfHasError · request entities) policies₁ policies₂ h₁
+
 theorem sound_policy_slice_is_equisatisfied (effect : Effect) (request : Request) (entities : Entities) (slice policies : Policies) :
-  slice ⊆ policies →
-  (∀ policy, policy ∈ policies → policy ∉ slice → ¬ satisfied policy request entities) →
+  IsSoundPolicySlice request entities slice policies →
   slice.filterMap (satisfiedWithEffect effect · request entities) ≡
   policies.filterMap (satisfiedWithEffect effect · request entities)
 := by
-  intros h₁ h₂
+  intro h
+  unfold IsSoundPolicySlice at h
+  have ⟨h₁, h₂⟩ := h; clear h
   simp [List.Equiv]
   simp [List.subset_def]
   apply And.intro <;>
   intros pid policy h₃ h₄ <;>
   apply Exists.intro policy <;>
   simp [h₄]
-  case _ =>
+  case left =>
     simp [List.subset_def] at h₁
     specialize h₁ h₃
     exact h₁
-  case _ =>
+  case right =>
     by_contra h₅
     specialize h₂ policy h₃ h₅
-    unfold satisfiedWithEffect at h₄
-    simp [h₂] at h₄
+    simp [h₂, satisfiedWithEffect] at h₄
 
 theorem satisfiedPolicies_eq_for_sound_policy_slice (effect : Effect) (request : Request) (entities : Entities) (slice policies : Policies) :
-  slice ⊆ policies →
-  (∀ policy, policy ∈ policies → policy ∉ slice → ¬ satisfied policy request entities) →
+  IsSoundPolicySlice request entities slice policies →
   satisfiedPolicies effect slice request entities = satisfiedPolicies effect policies request entities
 := by
-  intro h₁ h₂
+  intro h
   unfold satisfiedPolicies
   apply Set.make_eq_if_eqv
-  exact sound_policy_slice_is_equisatisfied effect request entities slice policies h₁ h₂
+  exact sound_policy_slice_is_equisatisfied effect request entities slice policies h
+
+theorem sound_policy_slice_is_equierror (request : Request) (entities : Entities) (slice policies : Policies) :
+  IsSoundPolicySlice request entities slice policies →
+  slice.filter (hasError · request entities) ≡ policies.filter (hasError · request entities)
+:= by
+  intro h
+  unfold IsSoundPolicySlice at h
+  have ⟨h₁, h₂⟩ := h; clear h
+  simp [List.Equiv, List.subset_def]
+  rw [List.subset_def] at h₁
+  apply And.intro <;>
+  intro policy <;>
+  simp [List.mem_filter] <;>
+  intro h₄ h₅ <;>
+  apply And.intro
+  case left.left => exact h₁ h₄
+  case left.right => exact h₅
+  case right.left =>
+    by_contra h₆
+    specialize h₂ policy h₄ h₆
+    exact h₂.right h₅
+  case right.right => exact h₅
+
+/--
+  an alternate, proved-equivalent, definition of errorPolicies that's easier to prove things about
+-/
+def alternateErrorPolicies (policies : Policies) (request : Request) (entities : Entities) : Set PolicyID :=
+  Set.make (List.map Policy.id (policies.filter (hasError · request entities)))
+
+theorem alternate_errorPolicies_equiv_errorPolicies {policies : Policies} {request : Request} {entities : Entities} :
+  errorPolicies policies request entities = alternateErrorPolicies policies request entities
+:= by
+  unfold errorPolicies alternateErrorPolicies
+  apply Set.make_eq_if_eqv
+  simp [List.Equiv, List.subset_def]
+  apply And.intro
+  case a.left =>
+    intro pid p h₁ h₂
+    apply Exists.intro p
+    unfold idIfHasError hasError at h₂
+    split at h₂
+    case inl h₃ =>
+      unfold hasError
+      apply And.intro
+      case left => simp [h₃, h₁, List.mem_filter]
+      case right => simp at h₂; exact h₂
+    case inr => contradiction
+  case a.right =>
+    intro p h₁
+    apply Exists.intro p
+    simp [List.mem_filter] at h₁
+    apply And.intro
+    case left => exact h₁.left
+    case right =>
+      unfold idIfHasError
+      split
+      case inl => rfl
+      case inr h₃ => simp [h₃] at h₁
+
+theorem errorPolicies_eq_for_sound_policy_slice (request : Request) (entities : Entities) (slice policies : Policies) :
+  IsSoundPolicySlice request entities slice policies →
+  errorPolicies slice request entities = errorPolicies policies request entities
+:= by
+  intro h
+  repeat rw [alternate_errorPolicies_equiv_errorPolicies]
+  unfold alternateErrorPolicies
+  apply Set.make_eq_if_eqv
+  apply List.map_equiv
+  exact sound_policy_slice_is_equierror request entities slice policies h
+
+theorem principal_eval_ok_means_principal_in_uid {policy : Policy} {request : Request} {entities : Entities} {uid: EntityUID} :
+  evaluate policy.principalScope.toExpr request entities = .ok true →
+  policy.principalScope.scope.bound = .some uid →
+  inₑ request.principal uid entities = true
+:= by
+  intro h₁ h₂
+  simp [PrincipalScope.toExpr, Scope.toExpr] at h₁
+  simp [Scope.bound, PrincipalScope.scope] at h₂
+  generalize h₃ : policy.principalScope.1 = x
+  rw [h₃] at h₁ h₂
+  cases x <;> simp at h₁ h₂ <;>
+  rw [h₂] at h₁
+  case eq =>
+    simp [evaluate, Var.eqEntityUID, apply₂] at h₁
+    simp [inₑ, h₁]
+  case mem =>
+    simp [evaluate, Var.inEntityUID, apply₂] at h₁
+    exact h₁
+  case isMem =>
+    replace h₁ := and_true_implies_right_true h₁
+    simp [evaluate, Var.inEntityUID, apply₂] at h₁
+    exact h₁
+
+theorem resource_eval_ok_means_resource_in_uid {policy : Policy} {request : Request} {entities : Entities} {uid : EntityUID} :
+  evaluate policy.resourceScope.toExpr request entities = .ok true →
+  policy.resourceScope.scope.bound = .some uid →
+  inₑ request.resource uid entities = true
+:= by
+  intro h₁ h₂
+  simp [ResourceScope.toExpr, Scope.toExpr] at h₁
+  simp [Scope.bound, ResourceScope.scope] at h₂
+  generalize h₃ : policy.resourceScope.1 = x
+  rw [h₃] at h₁ h₂
+  cases x <;> simp at h₁ h₂ <;>
+  rw [h₂] at h₁
+  case eq =>
+    simp [evaluate, Var.eqEntityUID, apply₂] at h₁
+    simp [inₑ, h₁]
+  case mem =>
+    simp [evaluate, Var.inEntityUID, apply₂] at h₁
+    exact h₁
+  case isMem =>
+    replace h₁ := and_true_implies_right_true h₁
+    simp [evaluate, Var.inEntityUID, apply₂] at h₁
+    exact h₁
 
 theorem satisfied_implies_principal_scope {policy : Policy} {request : Request} {entities : Entities} {uid : EntityUID} :
   satisfied policy request entities = true →
@@ -116,26 +252,9 @@ theorem satisfied_implies_principal_scope {policy : Policy} {request : Request} 
   inₑ request.principal uid entities = true
 := by
   intro h₁ h₂
-  simp [satisfied] at h₁
-  unfold Policy.toExpr at h₁
-  have h₃ := and_true_implies_left_true h₁
-  clear h₁
-  simp [PrincipalScope.toExpr, Scope.toExpr] at h₃
-  simp [Scope.bound, PrincipalScope.scope] at h₂
-  generalize h₄ : policy.3.1 = x
-  simp only [h₄] at h₂ h₃
-  cases x <;> simp at h₂ h₃ <;>
-  simp only [h₂] at h₃
-  case eq =>
-    simp [evaluate, Var.eqEntityUID, apply₂] at h₃
-    simp [inₑ, h₃]
-  case mem =>
-    simp [evaluate, Var.inEntityUID, apply₂] at h₃
-    exact h₃
-  case isMem =>
-    have h₅ := and_true_implies_right_true h₃
-    simp [evaluate, Var.inEntityUID, apply₂] at h₅
-    exact h₅
+  simp [satisfied, Policy.toExpr] at h₁
+  replace h₁ := and_true_implies_left_true h₁
+  exact principal_eval_ok_means_principal_in_uid h₁ h₂
 
 theorem satisfied_implies_resource_scope {policy : Policy} {request : Request} {entities : Entities} {uid : EntityUID} :
   satisfied policy request entities = true →
@@ -143,29 +262,347 @@ theorem satisfied_implies_resource_scope {policy : Policy} {request : Request} {
   inₑ request.resource uid entities = true
 := by
   intro h₁ h₂
-  simp [satisfied] at h₁
-  unfold Policy.toExpr at h₁
-  rcases
-    (and_true_implies_left_true
+  simp [satisfied, Policy.toExpr] at h₁
+  replace h₁ :=
+    and_true_implies_left_true
       (and_true_implies_right_true
-        (and_true_implies_right_true h₁))) with h₃
-  clear h₁
-  simp [ResourceScope.toExpr, Scope.toExpr] at h₃
-  simp [Scope.bound, ResourceScope.scope] at h₂
-  generalize h₄ : policy.5.1 = x
-  simp only [h₄] at h₂ h₃
-  cases x <;> simp at h₂ h₃ <;>
-  simp only [h₂] at h₃
-  case eq =>
-    simp [evaluate, Var.eqEntityUID, apply₂] at h₃
-    simp [inₑ, h₃]
-  case mem =>
-    simp [evaluate, Var.inEntityUID, apply₂] at h₃
-    exact h₃
-  case isMem =>
-    have h₅ := and_true_implies_right_true h₃
-    simp [evaluate, Var.inEntityUID, apply₂] at h₅
-    exact h₅
+        (and_true_implies_right_true h₁))
+  exact resource_eval_ok_means_resource_in_uid h₁ h₂
+
+/--
+  A generic lemma that relates List.mapM to List.map. Not in Std AFAICT.
+-/
+theorem if_f_produces_pure_then_mapM_f_is_pure_map {α β} [Monad m] [LawfulMonad m] {f : α → β} {list : List α} :
+  list.mapM ((fun a => pure (f a)) : α → m β) = pure (list.map f)
+:= by
+  induction list
+  case nil => simp
+  case cons x xs h => simp [h]
+
+/--
+  A generic lemma about composing List.mapM with List.map. Not in Std AFAICT.
+-/
+theorem mapM_over_map {α β γ} [Monad m] [LawfulMonad m] {f : α → β} {g : β → m γ} {list : List α} :
+  List.mapM g (list.map f) = list.mapM fun x => g (f x)
+:= by
+  induction list
+  case nil => simp
+  case cons x xs h => simp [h]
+
+theorem mapM_evaluate_uids_produces_uids {list : List EntityUID} {request : Request} {entities : Entities} :
+  List.mapM (evaluate · request entities) (list.map fun uid => Expr.lit (.entityUID uid)) = .ok (list.map (Value.prim ∘ Prim.entityUID))
+:= by
+  rw [mapM_over_map]
+  simp [evaluate]
+  apply if_f_produces_pure_then_mapM_f_is_pure_map
+
+theorem asEntityUID_of_uid {uid : EntityUID} :
+  Value.asEntityUID (.prim (.entityUID uid)) = .ok uid
+:= by
+  unfold Value.asEntityUID
+  split <;> simp
+  case h_1 uid' h => simp at h; simp [h]
+
+theorem mapM_asEntityUID_of_uid {uids : List EntityUID} :
+  List.mapM Value.asEntityUID (uids.map (Value.prim ∘ Prim.entityUID)) = .ok uids
+:= by
+  induction uids
+  case nil =>
+    rw [List.map_nil, List.mapM_nil]
+    simp [pure, Except.pure]
+  case cons x xs h_ind =>
+    rw [List.map_cons, List.mapM_cons]
+    simp [pure, Except.pure, asEntityUID_of_uid, h_ind]
+
+/--
+  A generic lemma about the behavior of List.mapM' in the Except monad
+-/
+theorem mapM'_ok_iff_f_ok_on_all_elements {f : α → Except ε β} {list : List α} :
+  Except.isOk (list.mapM' f) ↔ ∀ x ∈ list, Except.isOk (f x)
+:= by
+  simp [Except.isOk, Except.toBool]
+  constructor
+  case mp =>
+    induction list
+    case nil =>
+      intro _ x h₂
+      simp at h₂
+    case cons y ys h_ind =>
+      intro h₁ x h₂
+      unfold List.mapM' at h₁
+      cases h₄ : (f y) <;> simp [h₄] at h₁
+      case ok b =>
+        rcases (List.mem_cons.mp h₂) with h₅ | h₅
+        case inl => rw [← h₅] at h₄; simp [h₄]
+        case inr =>
+          apply h_ind; clear h_ind
+          case a =>
+            split at h₁ <;> split <;> simp
+            case h_1.h_2 h₅ _ _ h₆ => simp [h₆] at h₅
+            case h_2.h_2 => simp at h₁
+          case a => exact h₅
+  case mpr =>
+    induction list
+    case nil => simp [List.mapM', pure, Except.pure]
+    case cons x xs h_ind =>
+      intro h₂
+      split <;> simp
+      case h_2 err h₃ =>
+        cases h₄ : (f x) <;> simp [h₄] at h₂
+        case ok b =>
+          specialize h_ind h₂
+          split at h_ind <;> simp at h_ind
+          case h_1 err h₆ =>
+            simp [h₄, h₆, List.mapM', pure, Except.pure] at h₃
+
+theorem if_mapM'_doesn't_fail_on_list_then_doesn't_fail_on_set [LT α] [DecidableLT α] [StrictLT α] {f : α → Except ε β} {list : List α} :
+  Except.isOk (list.mapM' f) →
+  Except.isOk ((Set.elts (Set.make list)).mapM' f)
+:= by
+  simp [mapM'_ok_iff_f_ok_on_all_elements]
+  intro h₁ y h₂
+  apply h₁ y; clear h₁
+  apply Set.in_set_in_list' y list
+  exact Set.in_list_in_set y (Set.make list) h₂
+
+theorem mapM'_asEntityUID_on_set_uids_produces_ok {uids : List EntityUID} :
+  Except.isOk (List.mapM' Value.asEntityUID (Set.elts (Set.make (uids.map (Value.prim ∘ Prim.entityUID)))))
+:= by
+  apply if_mapM'_doesn't_fail_on_list_then_doesn't_fail_on_set
+  unfold Except.isOk Except.toBool
+  split <;> simp
+  case a.h_2 err h =>
+    rw [List.mapM'_eq_mapM] at h
+    simp [mapM_asEntityUID_of_uid] at h
+
+theorem mapOrErr_value_asEntityUID_on_uids_produces_set {list : List EntityUID} {err : Error} :
+  Set.mapOrErr Value.asEntityUID (Set.make (list.map (Value.prim ∘ Prim.entityUID))) err = .ok (Set.make list)
+:= by
+  unfold Set.mapOrErr
+  rw [←List.mapM'_eq_mapM]
+  split <;> simp
+  case h_1 list' h =>
+    -- in this case, mapping Value.asEntityUID over the set returns .ok
+    replace h := mapM'_asEntityUID_eq_entities h
+    have ⟨h₁, h₂⟩ := Set.elts_make_is_id_then_equiv h; clear h
+    apply Set.make_eq_if_eqv
+    unfold List.Equiv at *
+    repeat rw [List.subset_def] at *
+    constructor <;> intro a h₃ <;>
+    replace h₃ := List.mem_map_of_mem (Value.prim ∘ Prim.entityUID) h₃
+    case a.left =>
+      specialize h₁ h₃
+      simp at h₁
+      exact h₁
+    case a.right =>
+      specialize h₂ h₃
+      simp at h₂
+      exact h₂
+  case h_2 err h =>
+    -- in this case, mapping Value.asEntityUID over the set returns .error
+    have h₁ := @mapM'_asEntityUID_on_set_uids_produces_ok list
+    simp [h, Except.isOk, Except.toBool] at h₁
+
+theorem action_in_set_of_euids_produces_boolean {list : List EntityUID} {request : Request} {entities : Entities} :
+  producesBool (Expr.binaryApp BinaryOp.mem (Expr.var .action) (Expr.set (list.map fun uid => Expr.lit (.entityUID uid)))) request entities
+:= by
+  unfold producesBool
+  split <;> simp
+  case h_2 _ h =>
+    simp [evaluate, apply₂, inₛ] at h
+    rw [List.mapM₁_eq_mapM (evaluate · request entities)] at h
+    simp [mapM_evaluate_uids_produces_uids] at h
+    simp [mapOrErr_value_asEntityUID_on_uids_produces_set] at h
+
+/--
+  Lemma: evaluating the principalScope of any policy produces a boolean (and does not error)
+-/
+theorem principal_scope_produces_boolean {policy : Policy} {request : Request} {entities : Entities} :
+  producesBool policy.principalScope.toExpr request entities
+:= by
+  simp [producesBool, evaluate, PrincipalScope.toExpr, Scope.toExpr]
+  cases policy.principalScope.1 <;>
+  simp [evaluate, Var.eqEntityUID, Var.inEntityUID, Var.isEntityType, apply₁, apply₂]
+  case isMem ety uid =>
+    simp [Result.as, Lean.Internal.coeM, Coe.coe, Value.asBool, pure, Except.pure, CoeT.coe, CoeHTCT.coe, CoeHTC.coe, CoeOTC.coe, CoeTC.coe]
+    generalize (inₑ request.principal uid entities) = b₁
+    generalize (ety == request.principal.ty) = b₂
+    split <;> simp
+    case h_2 h => split at h <;> simp at h
+
+/--
+  Lemma: evaluating the actionScope of any policy produces a boolean (and does not error)
+-/
+theorem action_scope_produces_boolean {policy : Policy} {request : Request} {entities : Entities} :
+  producesBool policy.actionScope.toExpr request entities
+:= by
+  simp [producesBool, evaluate, ActionScope.toExpr, Scope.toExpr]
+  cases policy.actionScope
+  case actionInAny list =>
+    split <;> simp
+    case h_2 res h =>
+      simp at h
+      have h₁ := @action_in_set_of_euids_produces_boolean list request entities
+      unfold producesBool at h₁
+      split at h₁
+      case h_1 _ b h₂ => simp [h₂] at h
+      case h_2 => simp at h₁
+  case actionScope scope =>
+    simp [evaluate, Var.eqEntityUID, Var.inEntityUID, Var.isEntityType, apply₁, apply₂]
+    cases scope <;> simp [evaluate, apply₁, apply₂, Result.as]
+    case isMem ety uid =>
+      simp [Result.as, Lean.Internal.coeM, Coe.coe, Value.asBool, pure, Except.pure, CoeT.coe, CoeHTCT.coe, CoeHTC.coe, CoeOTC.coe, CoeTC.coe]
+      generalize (inₑ request.action uid entities) = b₁
+      generalize (ety == request.action.ty) = b₂
+      split <;> simp
+      case h_2 h => split at h <;> simp at h
+
+/--
+  Lemma: evaluating the resourceScope of any policy produces a boolean (and does not error)
+-/
+theorem resource_scope_produces_boolean {policy : Policy} {request : Request} {entities : Entities} :
+  producesBool policy.resourceScope.toExpr request entities
+:= by
+  simp [producesBool, evaluate, ResourceScope.toExpr, Scope.toExpr]
+  cases policy.resourceScope.1 <;>
+  simp [evaluate, Var.eqEntityUID, Var.inEntityUID, Var.isEntityType, apply₁, apply₂]
+  case isMem ety uid =>
+    simp [Result.as, Lean.Internal.coeM, Coe.coe, Value.asBool, pure, Except.pure, CoeT.coe, CoeHTCT.coe, CoeHTC.coe, CoeOTC.coe, CoeTC.coe]
+    generalize (inₑ request.resource uid entities) = b₁
+    generalize (ety == request.resource.ty) = b₂
+    split <;> simp
+    case h_2 h => split at h <;> simp at h
+
+/--
+  Lemma: if something produces a boolean, it does not produce a non-boolean
+-/
+theorem produces_boolean_means_not_non_boolean {e : Expr} {request : Request} {entities : Entities} :
+  producesBool e request entities → ¬ producesNonBool e request entities
+:= by
+  intro h₁
+  by_contra h₂
+  unfold producesBool at h₁
+  unfold producesNonBool at h₂
+  generalize (evaluate e request entities) = res at h₁ h₂
+  split at h₁
+  case h_1 => simp at h₂
+  case h_2 => split at h₂ <;> simp at h₁
+
+theorem principal_scope_does_not_throw {policy : Policy} {request : Request} {entities : Entities} {err : Error} :
+  ¬ (evaluate policy.principalScope.toExpr request entities = .error err)
+:= by
+  by_contra h
+  have h₁ := @principal_scope_produces_boolean policy request entities
+  simp [producesBool, h] at h₁
+
+theorem action_scope_does_not_throw {policy : Policy} {request : Request} {entities : Entities} {err : Error}:
+  ¬ (evaluate policy.actionScope.toExpr request entities = .error err)
+:= by
+  by_contra h
+  have h₁ := @action_scope_produces_boolean policy request entities
+  simp [producesBool, h] at h₁
+
+theorem resource_scope_does_not_throw {policy : Policy} {request : Request} {entities : Entities} {err : Error}:
+  ¬ (evaluate policy.resourceScope.toExpr request entities = .error err)
+:= by
+  by_contra h
+  have h₁ := @resource_scope_produces_boolean policy request entities
+  simp [producesBool, h] at h₁
+
+/--
+  For a policy to throw an error, we must have at least gotten past the scope,
+  so the scope constraints must have been satisfied.
+-/
+theorem error_implies_scope_satisfied {policy : Policy} {request : Request} {entities : Entities} {err : Error} :
+  evaluate policy.toExpr request entities = .error err →
+  evaluate policy.principalScope.toExpr request entities = .ok true ∧
+  evaluate policy.actionScope.toExpr request entities = .ok true ∧
+  evaluate policy.resourceScope.toExpr request entities = .ok true
+:= by
+  intro h₁
+  unfold Policy.toExpr at h₁
+  rcases (ways_and_can_error h₁) with h₂ | ⟨h₂, h₃⟩ | ⟨_, h₃⟩ | ⟨h₂, _, h₄⟩ <;> clear h₁
+  case _ =>
+    -- in this case, evaluating principal produced the error
+    exfalso; simp only [principal_scope_does_not_throw] at h₂
+  case _ =>
+    -- in this case, evaluating (action ∧ resource ∧ condition) produced the error
+    rcases (ways_and_can_error h₃) with h₄ | ⟨h₄, h₅⟩ | ⟨_, h₅⟩ | ⟨_, _, h₅⟩ <;> clear h₃
+    case _ =>
+      -- in this case, evaluating action produced the error
+      exfalso; simp only [action_scope_does_not_throw] at h₄
+    case _ =>
+      -- in this case, evaluating (resource ∧ condition) produced the error
+      rcases (ways_and_can_error h₅) with h₆ | ⟨h₆, _⟩ | ⟨_, h₇⟩ | ⟨_, h₇, _⟩ <;> clear h₅
+      case _ =>
+        -- in this case, evaluating resource produced the error
+        exfalso; simp only [resource_scope_does_not_throw] at h₆
+      case _ =>
+        -- in this case, evaluating condition produced the error
+        exact And.intro h₂ (And.intro h₄ h₆)
+      case _ =>
+        -- in this case, evaluating resource produced a non-boolean
+        exfalso
+        clear h₂
+        have h := @resource_scope_produces_boolean policy request entities
+        apply produces_boolean_means_not_non_boolean (e := policy.resourceScope.toExpr) h h₇
+      case _ =>
+        -- in this case, evaluating condition produced a non-boolean
+        exact And.intro h₂ (And.intro h₄ h₇)
+    case _ =>
+      -- in this case, evaluating action produced a non-boolean
+      exfalso
+      have h := @action_scope_produces_boolean policy request entities
+      apply produces_boolean_means_not_non_boolean (e := policy.actionScope.toExpr) h h₅
+    case _ =>
+      -- in this case, evaluating (resource ∧ condition) produced a non-boolean
+      exfalso
+      clear h₂
+      unfold producesNonBool at h₅
+      have h₄ := @and_produces_bool_or_error policy.resourceScope.toExpr policy.condition request entities
+      split at h₄ <;> simp at h₄
+      case _ h₆ => simp [h₆] at h₅
+      case _ h₆ => simp [h₆] at h₅
+  case _ =>
+    -- in this case, evaluating principal produced a non-boolean
+    exfalso
+    have h := @principal_scope_produces_boolean policy request entities
+    apply produces_boolean_means_not_non_boolean (e := policy.principalScope.toExpr) h h₃
+  case _ =>
+    -- in this case, evaluating (action ∧ resource ∧ condition) produced a non-boolean
+    exfalso
+    unfold producesNonBool at h₄
+    generalize (Expr.and policy.resourceScope.toExpr policy.condition) = resource_and_condition at h₂ h₄
+    have h₅ := @and_produces_bool_or_error policy.actionScope.toExpr resource_and_condition request entities
+    split at h₅ <;> simp at h₅
+    case _ h₆ => simp [h₆] at h₄
+    case _ h₆ => simp [h₆] at h₄
+
+/--
+  For a policy to throw an error, we must have at least gotten past the scope,
+  so the scope constraints must have been satisfied.
+-/
+theorem error_implies_principal_scope_in {policy : Policy} {request : Request} {entities : Entities} {uid : EntityUID} {err : Error} :
+  evaluate policy.toExpr request entities = .error err →
+  policy.principalScope.scope.bound = .some uid →
+  inₑ request.principal uid entities = true
+:= by
+  intro h₁ h₂
+  have ⟨hₚ, _, _⟩ := error_implies_scope_satisfied h₁
+  exact principal_eval_ok_means_principal_in_uid hₚ h₂
+
+/--
+  For a policy to throw an error, we must have at least gotten past the scope,
+  so the scope constraints must have been satisfied.
+-/
+theorem error_implies_resource_scope_in {policy : Policy} {request : Request} {entities : Entities} {uid : EntityUID} {err : Error} :
+  evaluate policy.toExpr request entities = .error err →
+  policy.resourceScope.scope.bound = .some uid →
+  inₑ request.resource uid entities = true
+:= by
+  intro h₁ h₂
+  have ⟨_, _, hᵣ⟩ := error_implies_scope_satisfied h₁
+  exact resource_eval_ok_means_resource_in_uid hᵣ h₂
 
 
 end Cedar.Thm
